Isabelle/01_Core/Refinement.thy
@@ -4,30 +4,30 @@ begin
 section \<open>Refines is preorder and order in regard to equivalence.\<close>
 
 
-lemma refines_is_reflexive: "p\<^sub>1 \<subseteq>\<^sub>p p\<^sub>1" \<comment> \<open>Refine_reflexive\<close>
+lemma refines_is_reflexive: "p\<^sub>1 \<sqsubseteq>\<^sub>p p\<^sub>1" \<comment> \<open>Refine_reflexive\<close>
   by (simp add: refines_def extends_def weakens_def strengthens_def restrict_r_def)
 
-lemma refines_is_transitive_e: "p\<^sub>1 \<subseteq>\<^sub>p p\<^sub>2 \<Longrightarrow> p\<^sub>2 \<subseteq>\<^sub>p p\<^sub>3 \<Longrightarrow> extends p\<^sub>1 p\<^sub>3"
+lemma refines_is_transitive_e: "p\<^sub>1 \<sqsubseteq>\<^sub>p p\<^sub>2 \<Longrightarrow> p\<^sub>2 \<sqsubseteq>\<^sub>p p\<^sub>3 \<Longrightarrow> extends p\<^sub>1 p\<^sub>3"
   by (auto simp: extends_def refines_def)
 
-lemma refines_is_transitive_w: "p\<^sub>1 \<subseteq>\<^sub>p p\<^sub>2 \<Longrightarrow> p\<^sub>2 \<subseteq>\<^sub>p p\<^sub>3 \<Longrightarrow> weakens p\<^sub>1 p\<^sub>3"
+lemma refines_is_transitive_w: "p\<^sub>1 \<sqsubseteq>\<^sub>p p\<^sub>2 \<Longrightarrow> p\<^sub>2 \<sqsubseteq>\<^sub>p p\<^sub>3 \<Longrightarrow> weakens p\<^sub>1 p\<^sub>3"
   by (auto simp: weakens_def refines_def)
 
-lemma refines_is_transitive_s: "p\<^sub>1 \<subseteq>\<^sub>p p\<^sub>2 \<Longrightarrow> p\<^sub>2 \<subseteq>\<^sub>p p\<^sub>3 \<Longrightarrow> strengthens p\<^sub>1 p\<^sub>3"
+lemma refines_is_transitive_s: "p\<^sub>1 \<sqsubseteq>\<^sub>p p\<^sub>2 \<Longrightarrow> p\<^sub>2 \<sqsubseteq>\<^sub>p p\<^sub>3 \<Longrightarrow> strengthens p\<^sub>1 p\<^sub>3"
   by (auto simp: strengthens_def weakens_def restrict_r_def refines_def)
 
-lemma refines_is_transitive: "p\<^sub>1 \<subseteq>\<^sub>p p\<^sub>2 \<Longrightarrow> p\<^sub>2 \<subseteq>\<^sub>p p\<^sub>3 \<Longrightarrow> p\<^sub>1 \<subseteq>\<^sub>p p\<^sub>3" \<comment> \<open>Refine_transitive\<close>
+lemma refines_is_transitive: "p\<^sub>1 \<sqsubseteq>\<^sub>p p\<^sub>2 \<Longrightarrow> p\<^sub>2 \<sqsubseteq>\<^sub>p p\<^sub>3 \<Longrightarrow> p\<^sub>1 \<sqsubseteq>\<^sub>p p\<^sub>3" \<comment> \<open>Refine_transitive\<close>
   by (metis refines_def refines_is_transitive_e refines_is_transitive_w refines_is_transitive_s)
 
-lemma refines_is_antisymetric: "p\<^sub>1 \<subseteq>\<^sub>p p\<^sub>2 \<Longrightarrow> p\<^sub>2 \<subseteq>\<^sub>p p\<^sub>1 \<Longrightarrow> p\<^sub>1 \<equiv>\<^sub>p p\<^sub>2" \<comment> \<open>Refine_antisym\<close>
+lemma refines_is_antisymetric: "p\<^sub>1 \<sqsubseteq>\<^sub>p p\<^sub>2 \<Longrightarrow> p\<^sub>2 \<sqsubseteq>\<^sub>p p\<^sub>1 \<Longrightarrow> p\<^sub>1 \<equiv>\<^sub>p p\<^sub>2" \<comment> \<open>Refine_antisym\<close>
   by (auto simp: refines_def extends_def weakens_def strengthens_def restrict_r_def equiv_def restr_post_def)
 
-theorem refines_is_preorder: "p\<^sub>1 \<subseteq>\<^sub>p p\<^sub>1 \<and> (p\<^sub>2 \<subseteq>\<^sub>p p\<^sub>3 \<and> p\<^sub>3 \<subseteq>\<^sub>p p\<^sub>4 \<longrightarrow> p\<^sub>2 \<subseteq>\<^sub>p p\<^sub>4)" \<comment> \<open>Refine_preorder\<close>
+theorem refines_is_preorder: "p\<^sub>1 \<sqsubseteq>\<^sub>p p\<^sub>1 \<and> (p\<^sub>2 \<sqsubseteq>\<^sub>p p\<^sub>3 \<and> p\<^sub>3 \<sqsubseteq>\<^sub>p p\<^sub>4 \<longrightarrow> p\<^sub>2 \<sqsubseteq>\<^sub>p p\<^sub>4)" \<comment> \<open>Refine_preorder\<close>
   apply (rule conjI)
   apply (rule refines_is_reflexive)
   using refines_is_transitive by auto
 
-theorem refines_is_order: "(p\<^sub>1 \<subseteq>\<^sub>p p\<^sub>1) \<and> (p\<^sub>2 \<subseteq>\<^sub>p p\<^sub>3 \<and> p\<^sub>3 \<subseteq>\<^sub>p p\<^sub>4 \<longrightarrow> p\<^sub>2 \<subseteq>\<^sub>p p\<^sub>4) \<and> (p\<^sub>5 \<subseteq>\<^sub>p p\<^sub>6 \<and> p\<^sub>6 \<subseteq>\<^sub>p p\<^sub>5 \<longrightarrow> p\<^sub>5 \<equiv>\<^sub>p p\<^sub>6)" \<comment> \<open>Refine_order\<close>
+theorem refines_is_order: "(p\<^sub>1 \<sqsubseteq>\<^sub>p p\<^sub>1) \<and> (p\<^sub>2 \<sqsubseteq>\<^sub>p p\<^sub>3 \<and> p\<^sub>3 \<sqsubseteq>\<^sub>p p\<^sub>4 \<longrightarrow> p\<^sub>2 \<sqsubseteq>\<^sub>p p\<^sub>4) \<and> (p\<^sub>5 \<sqsubseteq>\<^sub>p p\<^sub>6 \<and> p\<^sub>6 \<sqsubseteq>\<^sub>p p\<^sub>5 \<longrightarrow> p\<^sub>5 \<equiv>\<^sub>p p\<^sub>6)" \<comment> \<open>Refine_order\<close>
   using refines_is_antisymetric refines_is_preorder by blast
 
 theorem extends_is_reflexive: "extends p p"
