Isabelle/01_Core/Subprogram.thy
@@ -3,31 +3,31 @@ theory Subprogram
 begin
 section \<open>Subprogram for top.\<close>
 
-lemma subprogram_is_reflexive: "p\<^sub>1 \<preceq>\<^sub>p p\<^sub>1" \<comment> \<open>Subprogram_reflexive\<close>
-  by (simp add: subprogram_def extends_def weakens_def strengthens_def restrict_r_def)
+lemma specialize_is_reflexive: "p\<^sub>1 \<subseteq>\<^sub>p p\<^sub>1" \<comment> \<open>Subprogram_reflexive\<close>
+  by (simp add: specialize_def extends_def weakens_def strengthens_def restrict_r_def)
 
-lemma subprogram_is_transitive: "p\<^sub>1 \<preceq>\<^sub>p p\<^sub>2 \<Longrightarrow> p\<^sub>2 \<preceq>\<^sub>p p\<^sub>3 \<Longrightarrow> p\<^sub>1 \<preceq>\<^sub>p p\<^sub>3" \<comment> \<open>Subprogram_transitive\<close>
-  by (auto simp: subprogram_def extends_def weakens_def strengthens_def restrict_r_def subset_iff)
+lemma specialize_is_transitive: "p\<^sub>1 \<subseteq>\<^sub>p p\<^sub>2 \<Longrightarrow> p\<^sub>2 \<subseteq>\<^sub>p p\<^sub>3 \<Longrightarrow> p\<^sub>1 \<subseteq>\<^sub>p p\<^sub>3" \<comment> \<open>Subprogram_transitive\<close>
+  by (auto simp: specialize_def extends_def weakens_def strengthens_def restrict_r_def subset_iff)
 
-lemma subprogram_is_antisymetric: "p\<^sub>1 \<preceq>\<^sub>p p\<^sub>2 \<Longrightarrow> p\<^sub>2 \<preceq>\<^sub>p p\<^sub>1 \<Longrightarrow> p\<^sub>1 \<equiv>\<^sub>p p\<^sub>2" \<comment> \<open>Subprogram_antisym\<close>
-  by (auto simp: subprogram_def equiv_def extends_def weakens_def strengthens_def restrict_r_def restr_post_def)
+lemma specialize_is_antisymetric: "p\<^sub>1 \<subseteq>\<^sub>p p\<^sub>2 \<Longrightarrow> p\<^sub>2 \<subseteq>\<^sub>p p\<^sub>1 \<Longrightarrow> p\<^sub>1 \<equiv>\<^sub>p p\<^sub>2" \<comment> \<open>Subprogram_antisym\<close>
+  by (auto simp: specialize_def equiv_def extends_def weakens_def strengthens_def restrict_r_def restr_post_def)
 
-theorem subprogram_is_preorder: "p\<^sub>1 \<preceq>\<^sub>p p\<^sub>1 \<and> (p\<^sub>2 \<preceq>\<^sub>p p\<^sub>3 \<and> p\<^sub>3 \<preceq>\<^sub>p p\<^sub>4 \<longrightarrow> p\<^sub>2 \<preceq>\<^sub>p p\<^sub>4)" \<comment> \<open>Subprogram_preorder\<close>
+theorem specialize_is_preorder: "p\<^sub>1 \<subseteq>\<^sub>p p\<^sub>1 \<and> (p\<^sub>2 \<subseteq>\<^sub>p p\<^sub>3 \<and> p\<^sub>3 \<subseteq>\<^sub>p p\<^sub>4 \<longrightarrow> p\<^sub>2 \<subseteq>\<^sub>p p\<^sub>4)" \<comment> \<open>Subprogram_preorder\<close>
   apply (rule conjI)
-  apply (rule subprogram_is_reflexive)
-  using subprogram_is_transitive by auto
+  apply (rule specialize_is_reflexive)
+  using specialize_is_transitive by auto
 
-theorem subprogram_is_order: "(p\<^sub>1 \<preceq>\<^sub>p p\<^sub>1) \<and> (p\<^sub>2 \<preceq>\<^sub>p p\<^sub>3 \<and> p\<^sub>3 \<preceq>\<^sub>p p\<^sub>4 \<longrightarrow> p\<^sub>2 \<preceq>\<^sub>p p\<^sub>4) \<and> (p\<^sub>5 \<preceq>\<^sub>p p\<^sub>6 \<and> p\<^sub>6 \<preceq>\<^sub>p p\<^sub>5 \<longrightarrow> p\<^sub>5 \<equiv>\<^sub>p p\<^sub>6)" \<comment> \<open>Subprogram_order\<close>
-  using subprogram_is_antisymetric subprogram_is_preorder by blast
+theorem specialize_is_order: "(p\<^sub>1 \<subseteq>\<^sub>p p\<^sub>1) \<and> (p\<^sub>2 \<subseteq>\<^sub>p p\<^sub>3 \<and> p\<^sub>3 \<subseteq>\<^sub>p p\<^sub>4 \<longrightarrow> p\<^sub>2 \<subseteq>\<^sub>p p\<^sub>4) \<and> (p\<^sub>5 \<subseteq>\<^sub>p p\<^sub>6 \<and> p\<^sub>6 \<subseteq>\<^sub>p p\<^sub>5 \<longrightarrow> p\<^sub>5 \<equiv>\<^sub>p p\<^sub>6)" \<comment> \<open>Subprogram_order\<close>
+  using specialize_is_antisymetric specialize_is_preorder by blast
 
-theorem choice_decomp_1: "a \<preceq>\<^sub>p c \<and> b \<preceq>\<^sub>p c \<Longrightarrow> a \<union>\<^sub>p b \<preceq>\<^sub>p c"
-  apply (auto simp: subprogram_def)
+theorem choice_decomp_1: "a \<subseteq>\<^sub>p c \<and> b \<subseteq>\<^sub>p c \<Longrightarrow> a \<union>\<^sub>p b \<subseteq>\<^sub>p c"
+  apply (auto simp: specialize_def)
   apply (auto simp: extends_def choice_def restr_post_def restrict_r_def S_def Field_def) [1]
   apply (auto simp: weakens_def choice_def restr_post_def restrict_r_def S_def Field_def) [1]
   by (auto simp: strengthens_def choice_def restr_post_def restrict_r_def S_def Field_def) [1]
 
-theorem choice_decomp_2: "a \<union>\<^sub>p b \<preceq>\<^sub>p c \<Longrightarrow> a \<preceq>\<^sub>p c \<and> b \<preceq>\<^sub>p c"
-  apply (auto simp: subprogram_def)
+theorem choice_decomp_2: "a \<union>\<^sub>p b \<subseteq>\<^sub>p c \<Longrightarrow> a \<subseteq>\<^sub>p c \<and> b \<subseteq>\<^sub>p c"
+  apply (auto simp: specialize_def)
   apply (auto simp: extends_def choice_def restr_post_def restrict_r_def S_def Field_def) [1]
   apply (auto simp: weakens_def choice_def restr_post_def restrict_r_def S_def Field_def) [1]
   apply (auto simp: strengthens_def choice_def restr_post_def restrict_r_def S_def Field_def) [1]
@@ -35,14 +35,14 @@ theorem choice_decomp_2: "a \<union>\<^sub>p b \<preceq>\<^sub>p c \<Longrightar
   apply (auto simp: weakens_def choice_def restr_post_def restrict_r_def S_def Field_def) [1]
   by (auto simp: strengthens_def choice_def restr_post_def restrict_r_def S_def Field_def) [1]
 
-theorem choice_decomp: "a \<preceq>\<^sub>p c \<and> b \<preceq>\<^sub>p c \<equiv> a \<union>\<^sub>p b \<preceq>\<^sub>p c"
+theorem choice_decomp: "a \<subseteq>\<^sub>p c \<and> b \<subseteq>\<^sub>p c \<equiv> a \<union>\<^sub>p b \<subseteq>\<^sub>p c"
   by (smt (verit) choice_decomp_1 choice_decomp_2)
 
-theorem subprogram_equiv: "a \<preceq>\<^sub>p b \<Longrightarrow> a \<equiv>\<^sub>p c \<Longrightarrow> b \<equiv>\<^sub>p d \<Longrightarrow> c \<preceq>\<^sub>p d"
+theorem specialize_equiv: "a \<subseteq>\<^sub>p b \<Longrightarrow> a \<equiv>\<^sub>p c \<Longrightarrow> b \<equiv>\<^sub>p d \<Longrightarrow> c \<subseteq>\<^sub>p d"
   oops
 
-theorem equiv_subprogram_transitivity: "S a \<subseteq> S b \<Longrightarrow> S c \<subseteq> S d \<Longrightarrow> a \<equiv>\<^sub>p b \<Longrightarrow> b \<preceq>\<^sub>p c \<Longrightarrow> c \<equiv>\<^sub>p d \<Longrightarrow> a \<preceq>\<^sub>p d"
-  apply (auto simp: equiv_def subprogram_def)
+theorem equiv_specialize_transitivity: "S a \<subseteq> S b \<Longrightarrow> S c \<subseteq> S d \<Longrightarrow> a \<equiv>\<^sub>p b \<Longrightarrow> b \<subseteq>\<^sub>p c \<Longrightarrow> c \<equiv>\<^sub>p d \<Longrightarrow> a \<subseteq>\<^sub>p d"
+  apply (auto simp: equiv_def specialize_def)
   apply (auto simp: extends_def) [1]
   apply (auto simp: weakens_def) [1]
   by (auto simp: strengthens_def restrict_r_def restr_post_def) [1]
