Isabelle/02_Fundamental_operations/Corestriction.thy
@@ -24,23 +24,23 @@ lemma corestrict_prop_2: "Range_p (p \<setminus>\<^sub>p D) \<subseteq> Range_p 
 theorem corestrict_prop_: "Range_p (p \<setminus>\<^sub>p D) \<subseteq> Range_p p \<inter> D"
   by (auto simp: Range_p_def corestrict_p_def corestrict_r_def restrict_r_def)
 
-theorem NOT_corestricted_p_refines_p: "p \<setminus>\<^sub>p C \<subseteq>\<^sub>p p"
+theorem NOT_corestricted_p_refines_p: "p \<setminus>\<^sub>p C \<sqsubseteq>\<^sub>p p"
   oops \<comment> \<open>Not true as corestriction might remove a post relation completely\<close>
 
-theorem NOT_p_refines_corestricted_p: "p \<subseteq>\<^sub>p p \<setminus>\<^sub>p C"
+theorem NOT_p_refines_corestricted_p: "p \<sqsubseteq>\<^sub>p p \<setminus>\<^sub>p C"
   oops \<comment> \<open>Not true as corestriction might remove a post ambiguity\<close>
 
-theorem corestricted_refines_unrestricted_1: "p \<setminus>\<^sub>p C \<subseteq>\<^sub>p p" \<comment> \<open>T31\<close>
+theorem corestricted_refines_unrestricted_1: "p \<setminus>\<^sub>p C \<sqsubseteq>\<^sub>p p" \<comment> \<open>T31\<close>
   oops
-theorem unrestricted_refines_corestricted_1: "p \<subseteq>\<^sub>p p \<setminus>\<^sub>p C"
+theorem unrestricted_refines_corestricted_1: "p \<sqsubseteq>\<^sub>p p \<setminus>\<^sub>p C"
   oops
-theorem corestricted_refines_unrestricted_2: "is_feasible p \<Longrightarrow> p \<setminus>\<^sub>p C \<subseteq>\<^sub>p p"
+theorem corestricted_refines_unrestricted_2: "is_feasible p \<Longrightarrow> p \<setminus>\<^sub>p C \<sqsubseteq>\<^sub>p p"
   oops
-theorem unrestricted_refines_corestricted_2: "is_feasible p \<Longrightarrow> p \<subseteq>\<^sub>p p \<setminus>\<^sub>p C"
+theorem unrestricted_refines_corestricted_2: "is_feasible p \<Longrightarrow> p \<sqsubseteq>\<^sub>p p \<setminus>\<^sub>p C"
   oops
 
-theorem corestrict_subprog: "p \<setminus>\<^sub>p C \<preceq>\<^sub>p p" \<comment> \<open>Corestrict_subprog\<close>
-  by (auto simp: subprogram_def extends_def weakens_def restr_post_def corestrict_p_def corestrict_r_def restrict_r_def S_def Field_def strengthens_def)
+theorem corestrict_subprog: "p \<setminus>\<^sub>p C \<subseteq>\<^sub>p p" \<comment> \<open>Corestrict_subprog\<close>
+  by (auto simp: specialize_def extends_def weakens_def restr_post_def corestrict_p_def corestrict_r_def restrict_r_def S_def Field_def strengthens_def)
 
 theorem unrestricted_weakens_corestricted: "weakens p (p \<setminus>\<^sub>p C)"
   by (auto simp: weakens_def corestrict_p_def)
@@ -48,9 +48,9 @@ theorem unrestricted_weakens_corestricted: "weakens p (p \<setminus>\<^sub>p C)"
 theorem corestricted_strengthens_unrestricted: "strengthens (p \<setminus>\<^sub>p C) p"
   by (auto simp: strengthens_def corestrict_p_def restrict_r_def corestrict_r_def)
 
-theorem corestriction_prop: "D \<subseteq> C \<Longrightarrow> p \<setminus>\<^sub>p D \<subseteq>\<^sub>p p \<setminus>\<^sub>p C" \<comment> \<open>T32\<close>
+theorem corestriction_prop: "D \<subseteq> C \<Longrightarrow> p \<setminus>\<^sub>p D \<sqsubseteq>\<^sub>p p \<setminus>\<^sub>p C" \<comment> \<open>T32\<close>
   oops
-theorem corestriction_prop: "D \<subseteq> C \<Longrightarrow> p \<setminus>\<^sub>p C \<subseteq>\<^sub>p p \<setminus>\<^sub>p D" \<comment> \<open>T32\<close>
+theorem corestriction_prop: "D \<subseteq> C \<Longrightarrow> p \<setminus>\<^sub>p C \<sqsubseteq>\<^sub>p p \<setminus>\<^sub>p D" \<comment> \<open>T32\<close>
   oops
 
 theorem corestriction_weakens_prop: "D \<subseteq> C \<Longrightarrow> weakens (p \<setminus>\<^sub>p C) (p \<setminus>\<^sub>p D)"
@@ -59,8 +59,8 @@ theorem corestriction_weakens_prop: "D \<subseteq> C \<Longrightarrow> weakens (
 theorem corestriction_strengthens_prop: "D \<subseteq> C \<Longrightarrow> strengthens (p \<setminus>\<^sub>p D) (p \<setminus>\<^sub>p C)"
   by (auto simp: strengthens_def corestrict_p_def corestrict_r_def restrict_r_def)
 
-theorem corestrict_subprogorder1: "D \<subseteq> C \<Longrightarrow> (p \<setminus>\<^sub>p D) \<preceq>\<^sub>p (p \<setminus>\<^sub>p C)" \<comment> \<open>Corestrict_subprogorder1\<close>
-  by (auto simp: corestrict_p_def subprogram_def extends_def corestrict_r_def S_def Field_def weakens_def restr_post_def restrict_r_def strengthens_def)
+theorem corestrict_subprogorder1: "D \<subseteq> C \<Longrightarrow> (p \<setminus>\<^sub>p D) \<subseteq>\<^sub>p (p \<setminus>\<^sub>p C)" \<comment> \<open>Corestrict_subprogorder1\<close>
+  by (auto simp: corestrict_p_def specialize_def extends_def corestrict_r_def S_def Field_def weakens_def restr_post_def restrict_r_def strengthens_def)
 
 theorem equivalence_is_maintained_by_corestriction: "f\<^sub>1 \<equiv>\<^sub>p p\<^sub>1 \<Longrightarrow> (f\<^sub>1 \<setminus>\<^sub>p C) \<equiv>\<^sub>p p\<^sub>1 \<setminus>\<^sub>p C" \<comment> \<open>NEW\<close>
   by (auto simp: equiv_def restr_post_def restrict_r_def corestrict_p_def corestrict_r_def)
@@ -71,22 +71,22 @@ theorem equality_is_maintained_by_corestriction: "f\<^sub>1 \<triangleq> p\<^sub
 theorem corestrict_feasible: "is_feasible p \<Longrightarrow> is_feasible (p \<setminus>\<^sub>p C)" \<comment> \<open>Corestrict_feasible\<close>
   oops
 
-theorem corestriction_subsafety: "q \<preceq>\<^sub>p p \<Longrightarrow> q \<setminus>\<^sub>p C \<preceq>\<^sub>p p \<setminus>\<^sub>p C" \<comment> \<open>Corestriction_subsafety\<close>
-  by (auto simp: subprogram_def extends_def weakens_def strengthens_def restrict_r_def corestrict_p_def corestrict_r_def S_def Field_def Range_iff Domain_iff Un_def)
+theorem corestriction_subsafety: "q \<subseteq>\<^sub>p p \<Longrightarrow> q \<setminus>\<^sub>p C \<subseteq>\<^sub>p p \<setminus>\<^sub>p C" \<comment> \<open>Corestriction_subsafety\<close>
+  by (auto simp: specialize_def extends_def weakens_def strengthens_def restrict_r_def corestrict_p_def corestrict_r_def S_def Field_def Range_iff Domain_iff Un_def)
 
-theorem refinement_safety_corestriction: "q \<subseteq>\<^sub>p p \<Longrightarrow> q \<setminus>\<^sub>p C \<subseteq>\<^sub>p p \<setminus>\<^sub>p C" \<comment> \<open>Corestriction_refsafety\<close>
+theorem refinement_safety_corestriction: "q \<sqsubseteq>\<^sub>p p \<Longrightarrow> q \<setminus>\<^sub>p C \<sqsubseteq>\<^sub>p p \<setminus>\<^sub>p C" \<comment> \<open>Corestriction_refsafety\<close>
   oops
 
 theorem implements_safety_corestriction: "implements a b \<Longrightarrow> implements (a \<setminus>\<^sub>p C) (b \<setminus>\<^sub>p C)"
   oops
 
-theorem weakens_corestriction_1: "all_feasible [p, q] \<Longrightarrow> q \<subseteq>\<^sub>p p \<Longrightarrow> weakens (q \<setminus>\<^sub>p C) (p \<setminus>\<^sub>p C)" \<comment> \<open>Corestriction_refsafety\<close>
+theorem weakens_corestriction_1: "all_feasible [p, q] \<Longrightarrow> q \<sqsubseteq>\<^sub>p p \<Longrightarrow> weakens (q \<setminus>\<^sub>p C) (p \<setminus>\<^sub>p C)" \<comment> \<open>Corestriction_refsafety\<close>
   oops
-theorem weakens_corestriction_2: "q \<subseteq>\<^sub>p p \<Longrightarrow> weakens (p \<setminus>\<^sub>p C) (q \<setminus>\<^sub>p C)" \<comment> \<open>Corestriction_refsafety\<close>
+theorem weakens_corestriction_2: "q \<sqsubseteq>\<^sub>p p \<Longrightarrow> weakens (p \<setminus>\<^sub>p C) (q \<setminus>\<^sub>p C)" \<comment> \<open>Corestriction_refsafety\<close>
   oops
-theorem strengthens_corestriction_1: "q \<subseteq>\<^sub>p p \<Longrightarrow> strengthens (p \<setminus>\<^sub>p C) (q \<setminus>\<^sub>p C)" \<comment> \<open>Corestriction_refsafety\<close>
+theorem strengthens_corestriction_1: "q \<sqsubseteq>\<^sub>p p \<Longrightarrow> strengthens (p \<setminus>\<^sub>p C) (q \<setminus>\<^sub>p C)" \<comment> \<open>Corestriction_refsafety\<close>
   oops
-theorem strengthens_corestriction_2: "q \<subseteq>\<^sub>p p \<Longrightarrow> strengthens (q \<setminus>\<^sub>p C) (p \<setminus>\<^sub>p C)" \<comment> \<open>Corestriction_refsafety\<close>
+theorem strengthens_corestriction_2: "q \<sqsubseteq>\<^sub>p p \<Longrightarrow> strengthens (q \<setminus>\<^sub>p C) (p \<setminus>\<^sub>p C)" \<comment> \<open>Corestriction_refsafety\<close>
   by (auto simp: strengthens_def refines_def corestrict_p_def restrict_r_def corestrict_r_def)
 
 theorem corestrict_range_prop: "x \<in> C \<Longrightarrow> x \<notin> Range_p (p \<setminus>\<^sub>p C) \<Longrightarrow> x \<notin> Range_p (p)"
